prove that rose tree is also countable and start playing with hydra game

hol/countableListScript.sml
@@ -4,34 +4,187 @@ open arithmeticTheory rich_listTheory;
 
 val _ = new_theory "countableList";
 
-Theorem UNIV_list_BIGUNION:
-  (UNIV:'a list set) = BIGUNION (IMAGE (λk. {l | LENGTH l = k}) UNIV)
+Theorem EVERY_k_BIGUNION:
+  EVERY P = BIGUNION (IMAGE (λk. {l | EVERY P l ∧ LENGTH l = k}) UNIV)
 Proof
-  rw[EXTENSION,EQ_IMP_THM] >>
-  qexists `{l | LENGTH l = LENGTH x}` >>
-  simp[] >>
-  metis_tac[]
+  rw[EXTENSION,EQ_IMP_THM,IN_DEF] >>
+  gvs[] >>
+  qexists `{l | EVERY P l ∧ LENGTH l = LENGTH x}` >>
+  gvs[] >>
+  qexists `LENGTH x` >> fs[]
 QED
 
-Theorem set_SUC_LENGTH:
-  {l | LENGTH l = SUC k} = IMAGE (UNCURRY CONS) (UNIV × {l | LENGTH l = k})
+Theorem EVERY_SUC_k:
+  {l | EVERY P l ∧ LENGTH l = SUC k} =
+    IMAGE (UNCURRY CONS) (P × {l | EVERY P l ∧ LENGTH l = k})
 Proof
   rw[EXTENSION] >>
   Cases_on `x` >>
   gvs[ELIM_UNCURRY] >>
-  rw[EQ_IMP_THM,LAMBDA_PROD,GSYM PEXISTS_THM]
+  rw[EQ_IMP_THM,LAMBDA_PROD,GSYM PEXISTS_THM,IN_DEF]
+QED
+
+Theorem countable_EVERY:
+  countable P ⇒
+    countable (EVERY P)
+Proof
+  rw[Once EVERY_k_BIGUNION] >>
+  irule bigunion_countable >>
+  rw[IN_DEF] >>
+  Induct_on `k`
+  >- (
+    irule subset_countable >>
+    qexists `{[]}` >>
+    simp[SUBSET_DEF] ) >>
+  simp[EVERY_SUC_k]  >>
+  metis_tac[cross_countable,image_countable]
+QED
+
+Theorem EVERY_T:
+  EVERY (λx. T) = λl. T
+Proof
+  rw[FUN_EQ_THM]
 QED
 
 Theorem countable_list:
   countable (UNIV:'a set) ⇒
   countable (UNIV:'a list set)
 Proof
-  rw[UNIV_list_BIGUNION] >>
+  strip_tac >>
+  drule countable_EVERY >>
+  simp[UNIV_DEF,EVERY_T]
+QED
+
+Datatype:
+  Rose = Node 'a (Rose list)
+End
+
+Theorem Rose_size_def = fetch "-" "Rose_size_def";
+
+Definition rose_depth_def:
+  rose_depth (Node _ rs) = 1 + FOLDR MAX 0 (MAP rose_depth rs)
+Termination
+  WF_REL_TAC `measure (Rose_size (K 0))`
+End
+
+Theorem UNIV_rose_BIGUNION:
+  (UNIV:'a Rose set) = BIGUNION (IMAGE (λk. {r | rose_depth r = k}) UNIV)
+Proof
+  rw[EXTENSION,EQ_IMP_THM] >>
+  qexists `{r | rose_depth r = rose_depth x}` >>
+  simp[] >>
+  metis_tac[]
+QED
+
+Theorem rose_depth_0:
+  rose_depth r = 0 ⇔ F
+Proof
+  Cases_on `r` >> simp[rose_depth_def]
+QED
+
+Definition every_rose_def:
+  every_rose P (Node x rs) = (P x ∧ EVERY (every_rose P) rs)
+Termination
+  WF_REL_TAC `measure (Rose_size (K 0) o SND)`
+End
+
+Theorem every_rose_k_BIGUNION:
+  every_rose P = BIGUNION (IMAGE (λk. {r | every_rose P r ∧ rose_depth r ≤ k}) UNIV)
+Proof
+  rw[EXTENSION,EQ_IMP_THM,IN_DEF] >> gvs[] >>
+  qexists `{r | every_rose P r ∧ rose_depth r ≤ rose_depth x}` >>
+  gvs[] >>
+  qexists `rose_depth x` >> fs[]
+QED
+
+Theorem FOLDR_MAX_MEM:
+  ∀x xs. MEM x xs ⇒
+    x ≤ FOLDR MAX 0 xs
+Proof
+  Induct_on `xs` >> rw[] >>
+  rw[arithmeticTheory.LESS_EQ_REFL]
+QED
+
+Theorem FOLDR_MAX_LE:
+  (∀x. MEM x xs ⇒ x ≤ k) ⇒
+  FOLDR MAX 0 xs ≤ k
+Proof
+  Induct_on `xs` >> rw[]
+QED
+
+Theorem every_rose_SUC_k:
+  {r | every_rose P r ∧ rose_depth r ≤ SUC k} =
+    IMAGE (UNCURRY Node)
+      (P × {l | EVERY (λr. every_rose P r ∧ rose_depth r ≤ k) l})
+Proof
+  rw[EXTENSION] >>
+  qid_spec_tac `k` >>
+  qid_spec_tac `x` >>
+  ho_match_mp_tac rose_depth_ind >>
+  rw[every_rose_def,rose_depth_def] >>
+  rw[EQ_IMP_THM]
+  >- (
+    simp[LAMBDA_PROD,GSYM PEXISTS_THM,IN_DEF] >>
+    simp[EVERY_MEM] >>
+    rpt gen_tac >> strip_tac >>
+    last_x_assum $ qspec_then `r` (strip_assume_tac o iffRL) >>
+    gvs[PULL_EXISTS,ELIM_UNCURRY] >>
+    gvs[LAMBDA_PROD,GSYM PFORALL_THM,arithmeticTheory.ADD1] >>
+    gvs[EVERY_MEM] >>
+    irule arithmeticTheory.LESS_EQ_TRANS >>
+    last_assum $ irule_at (Pos last) >>
+    irule FOLDR_MAX_MEM >>
+    simp[MEM_MAP] >>
+    metis_tac[]
+  )
+  >- (Cases_on `x'` >> gvs[IN_DEF])
+  >- (
+    Cases_on `x'` >>
+    gvs[] >>
+    drule_at_then Any irule MONO_EVERY >>
+    rw[]
+  )
+  >- (
+    Cases_on `x'` >>
+    gvs[] >>
+    simp[arithmeticTheory.ADD1] >>
+    irule FOLDR_MAX_LE >>
+    rw[MEM_MAP] >>
+    gvs[EVERY_MEM]
+  )
+QED
+
+Theorem countable_every_rose:
+  countable P ⇒
+  countable (every_rose P)
+Proof
+  rw[Once every_rose_k_BIGUNION] >>
   irule bigunion_countable >>
-  rw[IN_DEF]
+  rw[IN_DEF] >>
   Induct_on `k` >>
-  simp[set_SUC_LENGTH] >>
-  metis_tac[cross_countable,image_countable]
+  simp[rose_depth_0,every_rose_SUC_k] >>
+  DEP_REWRITE_TAC[cross_countable,image_countable] >>
+  drule countable_EVERY >>
+  simp[GSPEC_ETA] >>
+  metis_tac[ETA_AX]
+QED
+
+Theorem every_rose_T:
+  every_rose (λx. T) = λr. T
+Proof
+  simp[FUN_EQ_THM] >>
+  `!P x. P = (λx. T) ⇒ every_rose P x` suffices_by gvs[] >>
+  ho_match_mp_tac every_rose_ind >>
+  rw[every_rose_def,EVERY_MEM]
+QED
+
+Theorem countable_rose:
+  countable (UNIV:'a set) ⇒
+  countable (UNIV:'a Rose set)
+Proof
+  strip_tac >>
+  drule countable_every_rose >>
+  simp[UNIV_DEF,every_rose_T]
 QED
 
 val _ = export_theory();
