hol/hydraScript.sml
@@ -1,0 +1,182 @@
+open HolKernel boolLib bossLib BasicProvers dep_rewrite;
+open pred_setTheory relationTheory listTheory pairTheory;
+open rich_listTheory;
+
+val _ = new_theory "hydra";
+
+(* part of the ideas are inspired by
+* "Hydra Battles in Coq" by Pierre Castéran
+* https://www.labri.fr/perso/casteran/hydras.pdf *)
+
+Datatype:
+  Rose = Node (Rose list)
+End
+
+Overload Leaf = ``Node []``;
+
+Inductive RemoveLeaf:
+[~head:]
+  RemoveLeaf (Leaf::rs) rs
+
+[~next:]
+  RemoveLeaf rs rs' ⇒ RemoveLeaf (r::rs) (r::rs')
+End
+
+Inductive RemoveRootLeaf:
+  RemoveLeaf rs rs' ⇒
+    RemoveRootLeaf (Node rs) (Node rs')
+End
+
+Theorem RemoveLeaf_append:
+  RemoveLeaf (xs  ++ Leaf::rs) (xs ++ rs)
+Proof
+  Induct_on `xs` >> rw[] >>
+  metis_tac[RemoveLeaf_rules]
+QED
+
+Theorem RemoveLeaf_exists_append:
+  ∀rs rs'. RemoveLeaf rs rs' ⇒
+  ∃xs y ys. rs = (xs  ++ Leaf::ys) ∧ rs' = (xs ++ ys)
+Proof
+  ho_match_mp_tac RemoveLeaf_ind >>
+  rw[]
+  >- (irule_at (Pos last) (GSYM $ cj 1 APPEND) >> simp[]) >>
+  irule_at (Pos last) (GSYM $ cj 2 APPEND) >> simp[]
+QED
+
+Inductive Spawn:
+[~head:]
+  RemoveRootLeaf t t' ⇒
+    Spawn (t::ts) (t'::(ts ++ REPLICATE n t'))
+[~next:]
+  Spawn ts ts' ⇒ Spawn (t::ts) (t::ts')
+End
+
+Inductive GenericSpawnNode:
+[~base:]
+  spawn ts ts' ⇒
+    GenericSpawnNode spawn (Node ts) (Node ts')
+
+[~head:]
+  GenericSpawnNode spawn t t' ⇒
+    GenericSpawnNode_l spawn (t::ts) (t'::ts)
+
+[~next:]
+  GenericSpawnNode_l spawn ts ts' ⇒
+    GenericSpawnNode_l spawn (t::ts) (t::ts')
+
+[~node:]
+  GenericSpawnNode_l spawn ts ts' ⇒
+    GenericSpawnNode spawn (Node ts) (Node ts')
+End
+
+Inductive SimpleSpawn:
+[~head:]
+  RemoveRootLeaf t t' ⇒
+    SimpleSpawn (t::ts) (t'::(ts ++ REPLICATE n Leaf))
+[~next:]
+  SimpleSpawn ts ts' ⇒ SimpleSpawn (t::ts) (t::ts')
+End
+
+Theorem Rose_size_def = fetch "-" "Rose_size_def";
+
+Definition default_EL_def:
+  default_EL d n l = if n < LENGTH l then EL n l else d
+End
+
+Overload EL0 = ``default_EL 0``;
+
+Definition LEX_LIST_def:
+  LEX_LIST cmp z (x::xs) (y::ys) =
+    (cmp x y ∨ (x = y ∧ LEX_LIST cmp z xs ys)) ∧
+  LEX_LIST cmp z [] (y::ys) = cmp z y ∧
+  LEX_LIST cmp z (x::xs) [] = cmp x z ∧
+  LEX_LIST cmp z _ _ = F
+End
+
+Definition Rose_depth_count_def:
+  Rose_depth_count_l ts = FLAT (MAP Rose_depth_count ts) ∧
+
+  Rose_depth_count (Node []) = [1n] ∧
+  Rose_depth_count (Node ts) =
+    MAP ($+ 1) $ Rose_depth_count_l ts
+Termination
+  WF_REL_TAC `measure 
+    (λt. case t of
+    | INL ts => Rose1_size ts
+    | INR n => Rose_size n)`
+End
+
+Triviality flip_flip:
+  flip (flip R) = R
+Proof
+  rw[FUN_EQ_THM]
+QED
+
+Triviality flip_TC_lem:
+  ∀x x'. (flip R)⁺ x x' ⇒ R⁺ x' x
+Proof
+  ho_match_mp_tac TC_INDUCT >>
+  rw[]
+  >- metis_tac[cj 1 TC_RULES]
+  >- metis_tac[cj 2 TC_RULES]
+QED
+
+Theorem flip_TC:
+  flip (TC R) = TC (flip R)
+Proof
+  rw[FUN_EQ_THM,EQ_IMP_THM,flip_TC_lem] >>
+  irule flip_TC_lem >>
+  simp[flip_flip]
+QED
+
+Theorem Rose_depth_count_positive:
+  (∀(ts:Rose list). EVERY (λx. 0 < x) (Rose_depth_count_l ts)) ∧ 
+  (∀(t:Rose). EVERY (λx. 0 < x) (Rose_depth_count t))
+Proof
+  ho_match_mp_tac Rose_depth_count_ind >>
+  rw[Rose_depth_count_def] >>
+  simp[EVERY_FLAT,EVERY_MAP,EVERY_MEM]
+QED
+
+Theorem LEX_FST_SND:
+  (f LEX g) p q ⇔ f (FST p) (FST q) ∨ (FST p = FST q ∧ g (SND p) (SND q))
+Proof
+  Cases_on `p` >>
+  Cases_on `q` >>
+  simp[LEX_DEF]
+QED
+
+
+Theorem SimpleSpawnNode_Rose_depth_count:
+  (∀ys xs.
+    GenericSpawnNode_l SimpleSpawn ys xs ⇒
+      _ (Rose_depth_count_l xs) (Rose_depth_count_l ys)) ∧
+  (∀y x.
+    GenericSpawnNode SimpleSpawn y x ⇒
+      _ (Rose_depth_count x) (Rose_depth_count y))
+Proof
+  ho_match_mp_tac GenericSpawnNode_ind >>
+  rw[Rose_depth_count_LEX_LT] >>
+  >- cheat
+  simp[
+QED
+
+Theorem WF_Simple_Hydra:
+  WF (flip $ GenericSpawnNode SimpleSpawn ∪ᵣRemoveRootLeaf)
+Proof
+  simp[flip_TC,WF_TC_EQN] >>
+  irule WF_SUBSET >>
+  qexists `inv_image _ Rose_depth_count` >>
+  reverse conj_tac
+  >- (
+    irule WF_inv_image >>
+    ntac 2 $ irule_at (Pos hd) WF_LEX >>
+    simp[]) >>
+  CONV_TAC SWAP_FORALL_CONV >>
+  simp[RUNION,DISJ_IMP_THM,FORALL_AND_THM] >>
+  conj_tac
+QED
+
+
+val _ = export_theory();
